Cslib/Computability/Machines/MultiTapeTuring/Routines/Typed.lean
@@ -25,8 +25,8 @@ public def computes_function {k : ℕ}
 public def computes_function_push {k : ℕ}
   {α : Type} [StrEnc α]
   (tm : MultiTapeTM k Char) (f : Data → α)
-  (i j : Fin k) (_h_neq : i ≠ j) :=
-  computes_function tm (fun tv d => tv.pushList (StrEnc.toData (f d))) i j _h_neq
+  (i j : Fin k) (h_neq : i ≠ j) :=
+  computes_function tm (fun tv d => tv.pushList (StrEnc.toData (f d))) i j h_neq
 
 /-- Turing machine `tm` computes a function of the current item at tape `i` seen as type
 -- `α` and pushes the result (type `β`) to tape `j`. -/
@@ -49,6 +49,15 @@ public def computes_function_update {k : ℕ}
   (views : Fin k → TapeView) :=
   tm.eval_struct views = some (Function.update views i ((views i).updateListHeadTyped f))
 
+@[simp]
+public theorem computes_function_seq {k : ℕ}
+  {β γ : Type} [StrEnc β] [StrEnc γ]
+  (tm₁ tm₂ : MultiTapeTM k Char) (f₁ : Data → β) (f₂ : β → γ)
+  (i j : Fin k) (h_neq : i ≠ j)
+  (h_comp₁ : ∀ views, computes_function_push tm₁ f₁ i j h_neq views)
+  (h_comp₂ : ∀ views, computes_function_update tm₂ f₂ i views)
+  (views : Fin k → TapeView) :
+  computes_function_push (tm₁ ;ₜ tm₂) (f₂ ∘ f₁) i j h_neq views := by sorry
 
 end Routines
 end Turing
